Tot interface for the alloc/dealloc-free fragment, with minimal additions to OrdSet; alloc/dealloc-fragment needs some more lemmas to be proved

examples/seplogic/SepLogic.Heap.fst
@@ -1,53 +1,51 @@
 module SepLogic.Heap
 
+module OS = FStar.OrdSet
+
+let addrs = OS.ordset nat (fun n m -> n <= m)
+
+unfold let disjoint_addrs (s0 s1:addrs) = OS.intersect s0 s1 = OS.empty
+
 private noeq type heap_rec = {
   next_addr : nat;
-  hdomain   : set nat;
+  hdomain   : addrs;
   memory    : nat -> Tot (option (a:Type0 & a))
 }
 
 let heap = h:heap_rec
   {(forall (r:nat) . 
-      S.mem r h.hdomain ==> r < h.next_addr) /\
-      (forall (r:nat) . S.mem r h.hdomain ==> Some? (h.memory r)) /\ 
-      (forall (r:nat) . S.mem r (S.complement h.hdomain) ==> None? (h.memory r))}
+      OS.mem r h.hdomain ==> r < h.next_addr) /\
+      (forall (r:nat) . OS.mem r h.hdomain ==> Some? (h.memory r)) /\ 
+      (forall (r:nat) . not (OS.mem r h.hdomain) ==> None? (h.memory r))}
 
 private let equal_heaps (h0 h1:heap) =
   let _ = () in
   h0.next_addr = h1.next_addr /\
-  S.equal h0.hdomain h1.hdomain /\ 
+  h0.hdomain = h1.hdomain /\ 
   FStar.FunctionalExtensionality.feq h0.memory h1.memory
-
-private let lemma_heap_ext (h0 h1:heap)
-  : Lemma (equal_heaps h0 h1 <==> h0 == h1)
-  = ()
   
 private noeq type memory_rec = {
-  domain   : set nat; 
+  domain   : addrs; 
   contents : nat -> Tot (option (a:Type0 & a))
 }
 
 let memory = m:(option memory_rec)
   {forall m' . m == Some m' ==> 
-               ((forall r . S.mem r m'.domain ==> Some? (m'.contents r)) /\ 
-                (forall r . S.mem r (S.complement m'.domain) ==> None? (m'.contents r)))}
+               ((forall r . OS.mem r m'.domain ==> Some? (m'.contents r)) /\ 
+                (forall r . not (OS.mem r m'.domain) ==> None? (m'.contents r)))}
 
 private let equal_memories (m0 m1:memory) =
   match (m0, m1) with
-  | (Some m0', Some m1') -> S.equal m0'.domain m1'.domain /\ 
+  | (Some m0', Some m1') -> m0'.domain = m1'.domain /\ 
                             FStar.FunctionalExtensionality.feq m0'.contents m1'.contents
   | (Some _, None)     -> False
   | (None, Some _)     -> False
   | (None, None)       -> True
 
-private let lemma_memory_ext (m0 m1:memory)
-  : Lemma (equal_memories m0 m1 <==> m0 == m1)
-  = ()
-
 let defined m = Some? m
 
 let emp = 
-  let domain = S.empty in
+  let domain = OS.empty in
   let contents = fun _ -> None in
   Some ({ domain = domain; contents = contents })
   
@@ -60,20 +58,20 @@ let heap_memory h = Some ({ domain   = h.hdomain;
 
 let disjoint_heaps (h0 h1:heap) =
   let _ = () in
-  S.disjoint h0.hdomain h1.hdomain
+  disjoint_addrs h0.hdomain h1.hdomain
 
 let join h0 h1 =
-  let domain = S.union h0.hdomain h1.hdomain in 
-  let memory = (fun r' ->  match (h0.memory r', h1.memory r') with
-                              | (Some v1, None) -> Some v1
-			      | (None, Some v2) -> Some v2
-			      | (None, None)    -> None) in
+  let domain = OS.union h0.hdomain h1.hdomain in 
+  let memory = (fun r ->  match (h0.memory r, h1.memory r) with
+                          | (Some v1, None) -> Some v1
+			  | (None, Some v2) -> Some v2
+			  | (None, None)    -> None) in
   if (h0.next_addr < h1.next_addr)
   then { next_addr = h1.next_addr; hdomain = domain; memory = memory }
   else { next_addr = h0.next_addr; hdomain = domain; memory = memory }
 
 let ( |> ) #a r x = 
-  let domain = S.singleton r in
+  let domain = OS.singleton r in
   let contents : nat -> Tot (option (a:Type0 & a)) = 
     (fun r' -> if r = r' then Some (| a , x |)
                          else None) in
@@ -82,8 +80,8 @@ let ( |> ) #a r x =
 let ( <*> ) m0 m1 = 
   match (m0, m1) with
   | (Some m0', Some m1') ->
-      (if (FStar.StrongExcludedMiddle.strong_excluded_middle (S.disjoint m0'.domain m1'.domain))
-       then (let domain = S.union m0'.domain m1'.domain in
+      (if (disjoint_addrs m0'.domain m1'.domain)
+       then (let domain = OS.union m0'.domain m1'.domain in
              let contents = (fun r -> match (m0'.contents r, m1'.contents r) with
                                      | (Some v1, None) -> Some v1
                                      | (None, Some v2) -> Some v2
@@ -124,12 +122,11 @@ let upd #a h r x = upd' h r x
 
 let fresh #a r h = 
   addr_of r >= h.next_addr
-  //h.memory r == None
 
 let alloc #a h0 x = 
   let r = h0.next_addr in 
   let next_addr = h0.next_addr + 1 in
-  let domain = S.union h0.hdomain (S.singleton r) in
+  let domain = OS.union h0.hdomain (OS.singleton r) in
   let memory = (fun r' -> if r = r' then Some (| a , x |)
                                     else h0.memory r') in
   let h1 = { next_addr = next_addr; hdomain = domain; memory = memory } in
@@ -137,14 +134,14 @@ let alloc #a h0 x =
 
 let dealloc #a h0 r =
   let next_addr = h0.next_addr in
-  let domain = S.intersect h0.hdomain (S.complement (S.singleton r)) in
+  let domain = OS.remove r h0.hdomain in
   let memory = (fun r' -> if r <> r' then h0.memory r'
                                      else None) in
   { next_addr = next_addr; hdomain = domain; memory = memory }
   
 let addrs_in m = 
   match m with
-  | Some m' -> m'.domain
+  | Some m' -> OS.as_set m'.domain
   | None    -> S.empty
 
 let addr_to_ref m r = 
@@ -153,23 +150,23 @@ let addr_to_ref m r =
     match m'.contents r with
     | Some v -> (| dfst v, r |)
 
-let restrict_memory rs m = 
-  match m with
+let restrict_memory rs m = admit ()
+  (*match m with
   | Some m' -> 
-      let domain = S.intersect rs m'.domain in 
-      let contents = (fun r -> if S.mem r domain 
+      let domain = OS.intersect_with_set m'.domain rs in 
+      let contents = (fun r -> if OS.mem r domain 
                                then m'.contents r
                                else None) in
-      Some ({ domain = domain; contents = contents })
+      Some ({ domain = domain; contents = contents })*)
 
-let complement_memory rs m = 
-  match m with 
+let complement_memory rs m = admit () //skipping this to do non alloc/dealloc parts first
+  (*match m with 
   | Some m' -> 
       let domain = S.intersect (S.complement rs) m'.domain in 
       let contents = (fun r -> if S.mem r domain
                                then m'.contents r
                                else None) in
-      Some ({ domain = domain; contents = contents })
+      Some ({ domain = domain; contents = contents })*)
 
 let lemma_disjoint_heaps_comm h0 h1 = ()
 
@@ -178,16 +175,46 @@ let lemma_disjoint_heaps_memories h0 h1 = ()
 let lemma_sep_defined_disjoint_heaps h0 h1 = ()
 
 let lemma_join_comm h0 h1 =
+  assert (OS.equal (OS.union h0.hdomain h1.hdomain) (OS.union h1.hdomain h0.hdomain));
   assert (equal_heaps (join h0 h1) (join h1 h0))
 
 let lemma_sep_unit m = 
-  assert (equal_memories (m <*> emp) m)
+  match m with 
+  | None    -> ()
+  | Some m' -> 
+      let (Some e) = emp in 
+      assert (OS.equal (OS.intersect m'.domain e.domain) OS.empty);
+      let (Some m'') = m <*> emp in 
+      assert (OS.equal m''.domain m'.domain);
+      assert (equal_memories (m <*> emp) m)
 
-let lemma_sep_comm m0 m1 = 
-  assert (equal_memories (m0 <*> m1) (m1 <*> m0))
+let lemma_sep_comm m0 m1 =
+  match (m0,m1) with
+  | (Some m0', Some m1') -> 
+      if (disjoint_addrs m0'.domain m1'.domain)
+      then (assert (OS.equal (OS.union m0'.domain m1'.domain) (OS.union m1'.domain m0'.domain));
+            let (Some m)  = m0 <*> m1 in
+            let (Some m') = m1 <*> m0 in
+            assert (equal_memories (m0 <*> m1) (m1 <*> m0)))
+      else (assert (equal_memories (m0 <*> m1) (m1 <*> m0)))
+  | _ -> ()
 
-let lemma_sep_assoc m0 m1 m2 =
-  assert (equal_memories (m0 <*> (m1 <*> m2)) ((m0 <*> m1) <*> m2))
+let lemma_sep_assoc m0 m1 m2 = 
+  match (m0,m1,m2) with
+  | (Some m0', Some m1', Some m2') -> 
+      if (disjoint_addrs m0'.domain m1'.domain && 
+          disjoint_addrs m1'.domain m2'.domain && 
+          disjoint_addrs m0'.domain m2'.domain)
+      then (assert (OS.equal (OS.union m0'.domain (OS.union m1'.domain m2'.domain)) 
+                             (OS.union (OS.union m0'.domain m1'.domain) m2'.domain));
+            assert (equal_memories (m0 <*> (m1 <*> m2)) ((m0 <*> m1) <*> m2)))
+      else if (not (disjoint_addrs m0'.domain m1'.domain))
+      then (assert (equal_memories (m0 <*> (m1 <*> m2)) ((m0 <*> m1) <*> m2)))
+      else if (not (disjoint_addrs m1'.domain m2'.domain))
+      then (assert (equal_memories (m0 <*> (m1 <*> m2)) ((m0 <*> m1) <*> m2)))
+      else if (not (disjoint_addrs m0'.domain m2'.domain))
+      then (assert (equal_memories (m0 <*> (m1 <*> m2)) ((m0 <*> m1) <*> m2)))
+  | _ -> ()
 
 let lemma_sep_join (h0 h1:heap) = 
   assert (equal_memories (heap_memory (join h0 h1)) 
@@ -226,9 +253,10 @@ let lemma_alloc_contains #a h0 x = ()
 
 let lemma_alloc_sel #a h0 x = ()
 
-let lemma_alloc_heap_memory #a h0 x =
-  let (r,h1) = alloc h0 x in 
-  assert (equal_memories (heap_memory h1) (heap_memory h0 <*> (r |> x)))
+let lemma_alloc_heap_memory #a h0 x = //TODO
+  admit ()
+  //let (r,h1) = alloc h0 x in 
+  //assert (equal_memories (heap_memory h1) (heap_memory h0 <*> (r |> x)))
 
 let lemma_fresh_in_complement #a r h = ()
 
@@ -236,8 +264,9 @@ let lemma_fresh_join #a r h0 h1 = ()
 
 let lemma_dealloc_contains #a h0 r = ()
 
-let lemma_points_to_dealloc #a h0 r = 
-  assert (equal_memories (heap_memory (dealloc h0 r)) emp)
+let lemma_points_to_dealloc #a h0 r = //TODO
+  admit ()
+  //assert (equal_memories (heap_memory (dealloc h0 r)) emp)
 
 let lemma_addrs_in_emp () = ()
 
@@ -249,10 +278,12 @@ let lemma_addrs_in_join m0 m1 = ()
 
 let lemma_addr_to_ref_addr_of m r = ()
 
-let lemma_restrict_complement_disjoint rs m = ()
+let lemma_restrict_complement_disjoint rs m = //TODO
+  admit ()
 
-let lemma_restrict_complement_sep rs m = 
-  assert (equal_memories m ((restrict_memory rs m) <*> (complement_memory rs m)))
+let lemma_restrict_complement_sep rs m = //TODO
+  admit ()
+  //assert (equal_memories m ((restrict_memory rs m) <*> (complement_memory rs m)))
 
 let lemma_fresh_or_old_refl h = 
   FStar.Classical.exists_intro (fun m -> fresh_or_old' h h (fst m) (snd m)) (heap_memory h,emp)
@@ -314,7 +345,8 @@ private let lemma_fresh_or_old_disjoint' (h0 h1 h2:heap) (m_old m_fresh:memory)
   : Lemma (requires (fresh_or_old' h0 h1 m_old m_fresh /\ 
                      disjoint_heaps h0 h2 /\ same_freshness h0 h2))
           (ensures  (disjoint_heaps h1 h2))
-  = assert (defined (m_old <*> m_fresh))
+  = admit () //TODO
+    //assert (defined (m_old <*> m_fresh))
 
 private let lemma_fresh_or_old_disjoint'' (h0 h1 h2:heap) (m_old m_fresh:memory)
   : Lemma (fresh_or_old' h0 h1 m_old m_fresh /\ 
